LocalAsGlobal.v
@@ -13,8 +13,6 @@ Parameter orD : forall {A}, D A -> D A -> D A.
 Parameter getD : forall {A}, (S -> D A) -> D A.
 Parameter putD : forall {A}, S -> D A -> D A.
 
-Parameter andD : forall {A}, D A -> D A -> D A.
-
 (* Laws *)
 
 Parameter get_get_G_D:
@@ -65,11 +63,11 @@ Parameter or_or_D:
   =
   orD p (orD q r).
 
-Parameter put_ret_or_G_D:
-  forall {A}  (v: S) (w: A) (q: D A),
-  putD v (orD (retD w) q)
-  =
-  andD (putD v (retD w)) (putD v q).
+Parameter put_ret_or_G_D':
+  forall {A} (v: S) (w: A) (q: D A),
+    putD v (orD (retD w) q)
+    =
+    orD (putD v (retD w)) (putD v q).
 
 End SemanticInterface.
 
@@ -81,7 +79,9 @@ Require Import Coq.Lists.List.
 Require Import Coq.Program.Equality.
 Require Import Coq.Logic.FunctionalExtensionality.
 
-(* Programs -- the free monad over the signature of fail + or + get + put *)
+(* Programs -- the free monad over the signature of fail + or + get + put.
+   These programs are closed, i.e. they contain no free variables.
+ *)
 Inductive Prog : Type -> Type :=
   | Return : forall {A}, A -> Prog A
   | Fail : forall {A}, Prog A
@@ -131,6 +131,7 @@ Qed.
 
 (* Programs with free variables *)
 
+(* Environment as a heterogeneous list *)
 Inductive Env : list Type -> Type :=
   | Nil : Env nil
   | Cons : forall {A L}, A -> Env L -> Env (A :: L).
@@ -151,6 +152,9 @@ Definition head_ {E} (env: Env E) :=
 
 Definition head {C E} (env: Env (C :: E)): C := head_ env.
 
+(* We represent open programs (programs with free variables) abstractly
+   as a function that produces a closed program when given an environment
+ *)
 Definition OProg (E: list Type)  (A: Type): Type := Env E -> Prog A.
 
 Definition comap {A E E'} (p: OProg E A) : (Env E' -> Env E) -> OProg E' A :=
@@ -182,92 +186,149 @@ Proof.
   intros; unfold obind, cpush, comap; auto.
 Qed.
 
-(* Contexts for open programs *)
+(* Contexts for open programs.
+   Predicates like (S -> bool) indicate control flow choices based on information
+   that is not statically available.
+   Context E1 A E2 B:
+           (E1, A) is the environment and return type of the whole
+           program,
+           (E2, B) is the environment and return type of the subprogram that is
+           expected in the hole.
+           So this context can be said to construct an open program that returns
+           a value of type A given an E1 environment, from an open program that
+           returns a value of type B given an E2 environment
+ *)
+ 
 Inductive Context : list Type -> Type -> list Type -> Type -> Type :=
-  | CHole   : forall {E A}, Context E A E A
-  | COr1    : forall {E1 E2 A B}, Context E1 A E2 B -> OProg E2 B -> Context E1 A E2 B
-  | COr2    : forall {E1 E2 A B}, OProg E2 B -> Context E1 A E2 B -> Context E1 A E2 B
-  | CPut     : forall {E1 E2 A B}, (Env E2 -> S) -> Context E1 A E2 B -> Context E1 A E2 B
-  | CGet     : forall {E1 E2 A B}, (S -> bool) -> (Context E1 A (S::E2) B) -> (S -> OProg E2 B)-> Context E1 A E2 B
-  | CDelay  : forall {E1 E2 A B}, (Env E2 -> bool) -> Context E1 A E2 B -> OProg E2 B -> Context E1 A E2 B
-  | CPush   : forall {E1 E2 A B C}, C -> Context E1 A (C::E2) B-> Context E1 A E2 B
-  | CLift      : forall {E1 E2 A B C}, Context E1 A E2 B -> Context E1 A (C::E2) B.
+  | CHole  : forall {E A        }, Context E A E A
 
-(* Applying a context to a program *)
+  | COr1   : forall {E1 E2 A B  }, Context E1 A E2 B ->
+                                   OProg E2 B ->
+                                   Context E1 A E2 B
+
+  | COr2   : forall {E1 E2 A B  }, OProg E2 B ->
+                                   Context E1 A E2 B ->
+                                   Context E1 A E2 B
+
+  | CPut   : forall {E1 E2 A B  }, (Env E2 -> S) ->
+                                   Context E1 A E2 B ->
+                                   Context E1 A E2 B
+
+  | CGet   : forall {E1 E2 A B  }, (S -> bool) ->
+                                   (Context E1 A (S::E2) B) ->
+                                   (S -> OProg E2 B) ->
+                                   Context E1 A E2 B
+
+  | CDelay : forall {E1 E2 A B  }, (Env E2 -> bool) ->
+                                   Context E1 A E2 B ->
+                                   OProg E2 B ->
+                                   Context E1 A E2 B
+
+  | CPush  : forall {E1 E2 A B C}, C ->
+                                   Context E1 A (C::E2) B ->
+                                   Context E1 A E2 B
+
+  | CLift  : forall {E1 E2 A B C}, Context E1 A E2 B ->
+                                   Context E1 A (C::E2) B.
+
+(* Applying a context to a program: produce a complete program from a program
+   containing a hole (a context) and a program to be filled into the hole.
+ *)
 Fixpoint appl {E1 E2: list Type} {A B: Type} (c: Context E1 A E2 B)  : OProg E1 A -> OProg E2 B :=
   match c in (Context E1 A E2 B) return (OProg E1 A -> OProg E2 B) with
-  | CHole => (fun p env => p env)
-  | COr1 c q => (fun p env => Or (appl c p env) (q env))
-  | COr2 p c => (fun q env => Or (p env) (appl c q env))
-  | CPut v c => (fun p env => Put (v env) (appl c p env)) 
-  | CGet t c q => (fun p env => Get (fun s => if t s then cpush s (appl c p) env else q s env))
+  | CHole        => (fun p env => p env)
+  | COr1 c q     => (fun p env => Or (appl c p env) (q env))
+  | COr2 p c     => (fun q env => Or (p env) (appl c q env))
+  | CPut v c     => (fun p env => Put (v env) (appl c p env)) 
+  | CGet t c q   => (fun p env => Get (fun s => if t s then cpush s (appl c p) env else q s env))
   | CDelay t c q => (fun p => (fun env => if t env then appl c p env else q env))
-  | CPush x c => (fun p env => cpush x (appl c p) env)
-  | CLift c => (fun p env => clift (appl c p) env) 
+  | CPush x c    => (fun p env => cpush x (appl c p) env)
+  | CLift c      => (fun p env => clift (appl c p) env) 
   end.
 
 (* Applying a context to a context, aka composing contexts *)
 Fixpoint applC {E1 E2 E3: list Type} {A B C: Type} (c: Context E2 B E3 C)  : Context E1 A E2 B -> Context E1 A E3 C:=
   match c in (Context E2 B E3 C) return (Context E1 A E2 B -> Context E1 A E3 C) with
-  | CHole => (fun d => d)
-  | COr1 c q => (fun d => COr1 (applC c d) q)
-  | COr2 p c => (fun d => COr2 p (applC c d))
-  | CPut v c => (fun d => CPut v (applC c d)) 
-  | CGet t c q => (fun d => CGet t (applC c d) q)
+  | CHole        => (fun d => d)
+  | COr1 c q     => (fun d => COr1 (applC c d) q)
+  | COr2 p c     => (fun d => COr2 p (applC c d))
+  | CPut v c     => (fun d => CPut v (applC c d)) 
+  | CGet t c q   => (fun d => CGet t (applC c d) q)
   | CDelay t c q => (fun d => CDelay t (applC c d) q)
-  | CPush x c => (fun d => CPush x (applC c d))
-  | CLift c => (fun d => CLift (applC c d))
+  | CPush x c    => (fun d => CPush x (applC c d))
+  | CLift c      => (fun d => CLift (applC c d))
   end.
 
-(* Alternative zipper-based context *)
+(* Alternative zipper-based context.
+   Whereas the Context datatype offers a top-down view of a program-with-hole,
+   the ZContext datatype offers a bottom-up view of a program-with-hole.
+
+   ZContext E1 A E2 B:
+            the hole has environment and type (E1,A); the ZContext
+            transforms a program of that type into a program of type B,
+            given environment E2.
+ *)
 Inductive ZContext : list Type -> Type -> list Type -> Type -> Type :=
-  | ZHole    : forall {E A}, ZContext E A E A
-  | ZOr1     : forall {E1 E2 A B}, ZContext E1 A E2 B -> OProg E1 A -> ZContext E1 A E2 B
-  | ZOr2     : forall {E1 E2 A B}, ZContext E1 A E2 B -> OProg E1 A -> ZContext E1 A E2 B
-  | ZPut      : forall {E1 E2 A B}, ZContext E1 A E2 B -> (Env E1 -> S) -> ZContext E1 A E2 B
-  | ZGet      : forall {E1 E2 A B}, ZContext E1 A E2 B -> (S -> bool) -> (S -> OProg E1 A) -> ZContext (S::E1) A E2 B
-  | ZDelay   : forall {E1 E2 A B}, ZContext E1 A E2 B -> (Env E1 -> bool) -> OProg E1 A -> ZContext E1 A E2 B
-  | ZPush    : forall {E1 E2 A B C}, ZContext E1 A E2 B -> C -> ZContext (C :: E1) A E2 B
-  | ZLift      : forall {E1 E2 A B C}, ZContext (C::E1) A E2 B -> ZContext E1 A E2 B.
+  | ZTop   : forall {E A},
+      ZContext E A E A
+
+  | ZOr1   : forall {E1 E2 A B},
+      ZContext E1 A E2 B -> OProg E1 A -> ZContext E1 A E2 B
+
+  | ZOr2   : forall {E1 E2 A B},
+      ZContext E1 A E2 B -> OProg E1 A -> ZContext E1 A E2 B
+
+  | ZPut   : forall {E1 E2 A B},
+      ZContext E1 A E2 B -> (Env E1 -> S) -> ZContext E1 A E2 B
+
+  | ZGet   : forall {E1 E2 A B},
+      ZContext E1 A E2 B -> (S -> bool) -> (S -> OProg E1 A) -> ZContext (S::E1) A E2 B
+
+  | ZDelay : forall {E1 E2 A B},
+      ZContext E1 A E2 B -> (Env E1 -> bool) -> OProg E1 A -> ZContext E1 A E2 B
+
+  | ZPush  : forall {E1 E2 A B C},
+      ZContext E1 A E2 B -> C -> ZContext (C :: E1) A E2 B
+
+  | ZLift  : forall {E1 E2 A B C},
+      ZContext (C::E1) A E2 B -> ZContext E1 A E2 B.
 
 Fixpoint zappl {E1 E2: list Type} {A B: Type} (z: ZContext E1 A E2 B)  : OProg E1 A -> OProg E2 B :=
   match z in (ZContext E1 A E2 B) return (OProg E1 A -> OProg E2 B) with
-  | ZHole => (fun p env => p env)
-  | ZOr1 z q => (fun p => zappl z (fun env => Or (p env) (q env)))
-  | ZOr2 z p => (fun q  => zappl z (fun env => Or (p env) (q env)))
-  | ZPut z v => (fun p => zappl z (fun env => Put (v env) (p env)))
-  | ZGet z t q => (fun p => zappl z (fun env => Get (fun s => if t s then (cpush s p) env else q s env)))
-  | ZDelay z t q => (fun p => zappl z (fun env => if t env then p env else q env))
-  | ZPush z c => (fun p => zappl z (cpush c p))
-  | ZLift z => (fun p => zappl z (clift p))
+  | ZTop         => (fun p env => p env)
+  | ZOr1 z q     => (fun p     => zappl z (fun env => Or (p env) (q env)))
+  | ZOr2 z p     => (fun q     => zappl z (fun env => Or (p env) (q env)))
+  | ZPut z v     => (fun p     => zappl z (fun env => Put (v env) (p env)))
+  | ZGet z t q   => (fun p     =>
+                       zappl z (fun env =>
+                                  Get (fun s => if t s
+                                                then (cpush s p) env
+                                                else q s env)))
+  | ZDelay z t q => (fun p     => zappl z (fun env => if t env then p env else q env))
+  | ZPush z c    => (fun p     => zappl z (cpush c p))
+  | ZLift z      => (fun p     => zappl z (clift p))
   end.
 
-Fixpoint toZContext_ {E1 E2 A B} (c: Context E1 A E2 B): (forall {E3 C}, ZContext E2 B E3 C-> ZContext E1 A E3 C) :=
-   match c in (Context E1 A E2 B) return ((forall {E3 C}, ZContext E2 B E3 C-> ZContext E1 A E3 C)) with
-   | CHole => (fun _ _ z => z)
-   | COr1 c p => (fun _ _ z => toZContext_ c (ZOr1 z p))
-   | COr2 p c => (fun _ _ z => toZContext_ c (ZOr2 z p))
-   | CPut s c => (fun _ _ z => toZContext_ c (ZPut z s))
-   | CGet t c p => (fun _ _ z => toZContext_ c (ZGet z t p))
+Fixpoint toZContext_ {E1 E2 A B} (c: Context E1 A E2 B):
+  (forall {E3 C}, ZContext E2 B E3 C-> ZContext E1 A E3 C) :=
+  match c in (Context E1 A E2 B) return ((forall {E3 C}, ZContext E2 B E3 C-> ZContext E1 A E3 C)) with
+   | CHole        => (fun _ _ z => z)
+   | COr1 c p     => (fun _ _ z => toZContext_ c (ZOr1 z p))
+   | COr2 p c     => (fun _ _ z => toZContext_ c (ZOr2 z p))
+   | CPut s c     => (fun _ _ z => toZContext_ c (ZPut z s))
+   | CGet t c p   => (fun _ _ z => toZContext_ c (ZGet z t p))
    | CDelay t c p => (fun _ _ z => toZContext_ c (ZDelay z t p))
-   | CPush a c => (fun _ _ z => toZContext_ c (ZPush z a))
-   | CLift c => (fun _ _ z => toZContext_ c (ZLift z))
+   | CPush a c    => (fun _ _ z => toZContext_ c (ZPush z a))
+   | CLift c      => (fun _ _ z => toZContext_ c (ZLift z))
   end.
 
-Definition toZContext {E1 E2 A B} (c: Context E1 A E2 B): ZContext E1 A E2 B := toZContext_ c ZHole.
-
+Definition toZContext {E1 E2 A B} (c: Context E1 A E2 B): ZContext E1 A E2 B := toZContext_ c ZTop.
+ 
 Lemma zappl_toZContext_:
    forall {E1 E2 A B} (c: Context E1 A E2 B) {E3 C} (z: ZContext E2 B E3 C) (p: OProg E1 A),
      zappl (toZContext_ c z) p = zappl z (appl c p).
 Proof.
-  intros E1 E2 A B c; induction c; intros E3 D z prog; simpl; auto.
-  - rewrite IHc; simpl; auto.
-  - rewrite IHc; simpl; auto.
-  - rewrite IHc; simpl; auto.
-  - rewrite IHc; simpl; auto.
-  - rewrite IHc; simpl; auto.
-  - rewrite IHc; simpl; auto.
-  - rewrite IHc; simpl; auto.
+  intros E1 E2 A B c; induction c; intros E3 D z prog; simpl; auto; rewrite IHc; auto.
 Qed.
 
 Lemma zappl_toZContext:
@@ -279,14 +340,14 @@ Qed.
 
 Fixpoint fromZContext_ {E2 E3: list Type} {B C: Type} (z: ZContext E2 B E3 C)  : forall {E1 A}, Context E1 A E2 B -> Context E1 A E3 C :=
   match z in (ZContext E2 B E3 C) return (forall {E1 A}, Context E1 A E2 B -> Context E1 A E3 C) with
-  | ZHole => (fun _ _ c => c)
-  | ZOr1 z q => (fun _ _ c => fromZContext_ z (COr1 c q)) 
-  | ZOr2 z p => (fun _ _ c => fromZContext_ z (COr2 p c))
-  | ZPut z v => (fun _ _ c => fromZContext_ z (CPut v c))
-  | ZGet z t q => (fun _ _ c =>fromZContext_ z (CGet t c q))
+  | ZTop         => (fun _ _ c => c)
+  | ZOr1 z q     => (fun _ _ c => fromZContext_ z (COr1 c q)) 
+  | ZOr2 z p     => (fun _ _ c => fromZContext_ z (COr2 p c))
+  | ZPut z v     => (fun _ _ c => fromZContext_ z (CPut v c))
+  | ZGet z t q   => (fun _ _ c => fromZContext_ z (CGet t c q))
   | ZDelay z t q => (fun _ _ c => fromZContext_ z (CDelay t c q))
-  | ZPush z x => (fun _ _ c => fromZContext_ z (CPush x c))
-  | ZLift z => (fun _ _ c => fromZContext_ z (CLift c))
+  | ZPush z x    => (fun _ _ c => fromZContext_ z (CPush x c))
+  | ZLift z      => (fun _ _ c => fromZContext_ z (CLift c))
   end.
 
 Definition fromZContext {E1 E2: list Type}  {A B: Type} (z: ZContext E1 A E2 B)  : Context E1 A E2 B :=
@@ -296,37 +357,21 @@ Lemma  appl_fromZContext_:
   forall {B C E2 E3} (z: ZContext E2 B E3 C) {E1 A} (c: Context E1 A E2 B) (p: OProg E1 A),
        appl (fromZContext_ z c) p = zappl z (appl c p).
 Proof.
-  intros B C E2 E3 z; induction z; intros E0 A0 c0 p; simpl.
-  - auto.
-  - rewrite IHz; simpl; auto.
-  - rewrite IHz; simpl; auto.
-  - rewrite IHz; simpl; auto.
-  - rewrite IHz; simpl; auto.
-  - rewrite IHz; simpl; auto.
-  - rewrite IHz; simpl; auto.
-  - rewrite IHz; simpl; auto.
+  intros B C E2 E3 z; induction z; intros E0 A0 c0 p; auto; simpl; rewrite IHz; auto.
 Qed.
 
 Lemma  appl_fromZContext:
   forall {A B E1 E2} (z: ZContext E1 A E2 B) (p: OProg E1 A),
        appl (fromZContext z) p = zappl z p.
 Proof.
-  intros; unfold fromZContext; rewrite appl_fromZContext_; simpl; auto.
+  intros; unfold fromZContext; rewrite appl_fromZContext_; auto.
 Qed.
 
 Lemma toZContext_fromZContext_:
   forall {E2 E3 B C} (z: ZContext E2 B E3 C) {E1 A} (c: Context E1 A E2 B),
   toZContext (fromZContext_ z c) = toZContext_ c z.
 Proof.
-  intros E2 E3 B C z; induction z; intros E0 A0 c0.
-  - simpl; auto.
-  - simpl; rewrite IHz; simpl; auto.
-  - simpl; rewrite IHz; simpl; auto.
-  - simpl; rewrite IHz; simpl; auto.
-  - simpl; rewrite IHz; simpl; auto.
-  - simpl; rewrite IHz; simpl; auto.
-  - simpl; rewrite IHz; simpl; auto.
-  - simpl; rewrite IHz; simpl; auto.
+  intros E2 E3 B C z; induction z; intros E0 A0 c0; simpl; auto; rewrite IHz; auto.
 Qed. 
 
 Lemma toZContext_fromZContext:
@@ -343,6 +388,9 @@ Inductive Concat : list Type -> list Type -> list Type -> Type :=
 
 Fixpoint concat_nil_r  {E}: Concat E E nil :=
   match E with
+
+
+
   | nil     => CNil nil
   | X::Xs => CCons X Xs Xs nil (concat_nil_r)
   end.
@@ -353,6 +401,31 @@ Fixpoint appendEnv_ {E1} (env: Env E1): forall E2, Env E2 -> Env (E1 ++ E2) :=
   end.
 *)
 
+(*
+Inductive Prog : Type -> Type :=
+  | Return : forall {A}, A -> Prog A
+  | Fail : forall {A}, Prog A
+  | Or : forall {A}, Prog A -> Prog A -> Prog A
+  | Get : forall {A}, (S -> Prog A) ->Prog A
+  | Put : forall {A}, S -> Prog A ->Prog A.
+
+(* The algebra for the signature *)
+Parameter retD: forall {A}, A -> D A.
+Parameter failD : forall {A}, D A.
+Parameter orD : forall {A}, D A -> D A -> D A.
+Parameter getD : forall {A}, (S -> D A) -> D A.
+Parameter putD : forall {A}, S -> D A -> D A.
+*)
+Fixpoint run {A} (p : Prog A) : D A :=
+  match p with
+  | Return x => retD x
+  | Fail     => failD
+  | Or p q   => orD (run p) (run q)
+  | Get p    => getD (fun s => run (p s))
+  | Put s p  => putD s (run p)
+  end.
+
+(*
 (* The semantic function for global, i.e. non-backtracking, state *)
 Parameter run : forall {A}, Prog A -> D A.
 
@@ -362,36 +435,55 @@ Parameter run_fail: forall {A}, @run A Fail = failD.
 Parameter run_or: forall {A} (p q: Prog A), run (Or p q) = orD (run p) (run q).
 Parameter run_get: forall {A} (p: S -> Prog A),     run (Get p) = getD (fun s => run (p s)).
 Parameter run_put:forall {A} (s: S) (p: Prog A), run (Put s p) = putD s (run p).
+*)
+
+Lemma run_ret: forall {A} (x: A), run (Return x) = retD x.
+Proof. auto. Qed.
+
+Lemma run_fail: forall {A}, @run A Fail = failD.
+Proof. auto. Qed.
+
+Lemma run_or : forall {A} (p q : Prog A), run (Or p q) = orD (run p) (run q).
+Proof. auto. Qed.
+
+Lemma run_get: forall {A} (p: S -> Prog A), run (Get p) = getD (fun s => run (p s)).
+Proof. auto. Qed.
+
+Lemma run_put:forall {A} (s: S) (p: Prog A), run (Put s p) = putD s (run p).
+Proof. auto. Qed.
 
 (* Derived definitions for open programs *)
-Definition orun : forall {A E}, OProg E A -> Env E -> D A := fun _ _ p env => run (p env).
+Definition orun : forall {A E}, OProg E A -> Env E -> D A :=
+  fun _ _ p env => run (p env).
 
 Lemma orun_fail:
   forall {A E},
     @orun A E (fun env => Fail) = fun _ => failD.
 Proof.
-  intros; apply functional_extensionality; intro env;  unfold orun; auto using run_fail.
+  intros. apply functional_extensionality. intro env. 
+  unfold orun.
+  auto.
 Qed.
 
 Lemma orun_or:
   forall {A E} (p q: OProg E A),
     orun (fun env => Or (p env) (q env)) = fun env => orD (orun p env) (orun q env).
 Proof.
-  intros; apply functional_extensionality; intro env; unfold orun. auto using run_or.
+  intros; apply functional_extensionality; intro env; unfold orun. auto.
 Qed.
 
 Lemma orun_get:
   forall {A E} (p: S -> OProg E A),
     orun (fun env => Get (fun s => p s env)) = fun env => getD (fun s => orun (p s) env).
 Proof.
-  intros; apply functional_extensionality; intro env; unfold orun; auto using run_get.
+  intros; apply functional_extensionality; intro env; unfold orun; auto.
 Qed.
 
 Lemma orun_put:
   forall {E A} (s: Env E -> S) (p: OProg E A),
     orun (fun env => Put (s env) (p env)) = fun env => putD (s env) (orun p env).
 Proof.
-  intros; apply functional_extensionality; intro env; unfold orun; auto using run_put.
+  intros; apply functional_extensionality; intro env; unfold orun; auto.
 Qed.
 
 Lemma get_get_G':
@@ -400,14 +492,7 @@ Lemma get_get_G':
     =
     run (Get (fun s => k s s)).
 Proof.
-  intros A k.
-  repeat rewrite run_get.
-  erewrite (@f_equal _ _ _ _ (fun s : S => getD (fun s' : S => run (k s s'))) _).
-  - rewrite get_get_G_D.
-  reflexivity.
-  Unshelve.
-  apply functional_extensionality; intro s0.
-  rewrite run_get; auto.
+  intros A k. simpl. apply get_get_G_D.
 Qed.
 
 Lemma meta_G:
@@ -419,27 +504,47 @@ Lemma meta_G:
     = 
     orun (appl c (fun env => q (f env))).
 Proof.
-  intros A B E1 E2 X p q meta_G' f c; induction c; simpl.
-  - unfold orun; apply functional_extensionality; intro env0; apply meta_G'.
-  - repeat rewrite orun_or; apply functional_extensionality; intro env; rewrite (IHc p q); auto.
-  - repeat rewrite orun_or; apply functional_extensionality; intro env0; rewrite  (IHc p q); auto.
-  - repeat rewrite orun_put; apply functional_extensionality; intro env0; rewrite (IHc p q); auto.
-  - repeat rewrite orun_get; apply functional_extensionality; intro env0;
-     apply f_equal; apply functional_extensionality; intro s0; destruct (b s0);
-     [ unfold cpush, comap; change (orun (fun env => appl c ?p (Cons s0 env)) env0) with
-                (orun (appl c p) (Cons s0 env0)); rewrite  (IHc p q); auto | auto ].
-  - change (orun ?f) with (fun env => orun f env); apply functional_extensionality; intro env0;
-     change (orun (fun env => if b env then ?f env else ?g env) env0) with
-                 (orun (fun env => if b env0 then f env else g env) env0); destruct (b env0);
-    [ change (fun env => appl c ?p env) with (appl c p); rewrite (IHc p q); auto | auto ].
-  - unfold cpush, comap; change (orun (fun env => appl c0 ?p (Cons c env))) with
-                                                   (fun env => orun (appl c0 p) (Cons c env));
-    apply functional_extensionality; intro env0; rewrite (IHc p q); auto.
- - unfold clift, comap;
-   change (orun (fun env => appl c ?p (tail env))) with
-               (fun env => orun (appl c p) (@tail C _ env));
-   apply functional_extensionality; intro env0; rewrite (IHc p q);
-  auto.
+  intros.
+  induction c; simpl.
+  - unfold orun.
+    apply functional_extensionality.
+    simpl.
+    intro env0.
+    apply meta_G'.
+  - repeat rewrite orun_or. rewrite (IHc p q); auto.
+  - repeat rewrite orun_or. rewrite (IHc p q); auto.
+  - repeat rewrite orun_put. rewrite (IHc p q); auto.
+  - repeat rewrite orun_get.
+    apply functional_extensionality; intro env.
+    f_equal. apply functional_extensionality; intro s; destruct (b s).
+    + unfold cpush. unfold comap.
+      assert (H : forall r,
+                 orun (fun env => appl c r (Cons s env))
+                 =
+                 fun env => orun (appl c r) (Cons s env)).
+      { auto. }
+      rewrite H.
+      rewrite IHc with (q:=q).
+      auto.
+      apply meta_G'.
+    + reflexivity.
+  - change (orun ?f) with (fun env => orun f env);
+    apply functional_extensionality; intro env0.
+    change (orun (fun env => if b env then ?f env else ?g env) env0) with
+        (orun (fun env => if b env0 then f env else g env) env0).
+    destruct (b env0).
+    + rewrite IHc with (q:=q).
+      auto.
+      apply meta_G'.
+    + reflexivity.
+  - unfold cpush, comap.
+    change (orun (fun env => appl c0 ?r (Cons c env)))
+      with (fun env => orun (appl c0 r) (Cons c env)).
+    rewrite IHc with (q:=q); auto.
+  - unfold clift, comap.
+    change (orun (fun env => appl c ?r (tail env)))
+      with (fun env => orun (appl c r) (@tail C _ env)).
+    rewrite IHc with (q:=q); auto.
 Qed.
 
 Lemma get_get_G:
@@ -463,10 +568,8 @@ Lemma get_put_G':
    =
    run q.
 Proof.
-  intros; rewrite run_get.
-  assert ((fun s => run (Put s q)) = (fun s => putD s (run q))).
-  apply functional_extensionality; intros s; rewrite run_put; auto.
-  rewrite H; rewrite get_put_G_D; reflexivity.
+  intros.
+  apply get_put_G_D.
 Qed.
 
 Lemma get_put_G:
@@ -490,7 +593,7 @@ Lemma put_get_G':
     =
     run (Put s (p s)).
 Proof.
-  intros; rewrite run_put, run_get, run_put.
+  intros. simpl.
   apply (put_get_G_D s (fun s => run (p s))).
 Qed.
 
@@ -539,7 +642,7 @@ Lemma put_or_G':
    = 
    run (Put s (Or p q)).
 Proof.
-  intros; repeat rewrite run_put, run_or; apply put_or_G_D.
+  intros; apply put_or_G_D.
 Qed.
 
 Lemma put_or_G:
@@ -563,7 +666,7 @@ Lemma or_fail':
     =
     run q.
 Proof.
-  intros; repeat rewrite run_or,run_fail; apply or1_fail_D.
+  intros; apply or1_fail_D.
 Qed.
 
 Lemma or_fail:
@@ -587,7 +690,7 @@ Lemma  fail_or':
     =
     run q.
 Proof.
-  intros; repeat rewrite run_or,run_fail; apply or2_fail_D.
+  intros; apply or2_fail_D.
 Qed.
 
 Lemma fail_or:
@@ -611,7 +714,7 @@ Lemma or_or':
     =
     run (Or p (Or q r)).
 Proof.
-  intros; repeat rewrite run_or; apply or_or_D.
+  intros; apply or_or_D.
 Qed.
 
 Lemma or_or:
@@ -633,22 +736,20 @@ Lemma put_ret_or_G:
   forall {A} (v: S) (w: A) (q: Prog A),
   run (Put v (Or (Return w) q))
   =
-  andD (run (Put v (Return w))) (run (Put v q)).
+  run (Or (Put v (Return w)) (Put v q)).
 Proof.
-  intros. repeat rewrite run_put.
-  rewrite run_or.
-  repeat rewrite run_ret.
-  apply put_ret_or_G_D.
+  intros.
+  apply put_ret_or_G_D'.
 Qed.
 
-(* Translating the syntx of local state semantics programs to global state semantics programs *)
+(* Translating the syntax of local state semantics programs to global state semantics programs *)
 Fixpoint trans {A} (p: Prog A): Prog A :=
   match p with
   | Return x => Return x
-  | Or p q => Or (trans p) (trans q)
-  | Fail => Fail
-  | Get p => Get (fun s => trans (p s))
-  | Put s p => Get (fun s0 => Or (Put s (trans p)) (Put s0 Fail))
+  | Or p q   => Or (trans p) (trans q)
+  | Fail     => Fail
+  | Get p    => Get (fun s => trans (p s))
+  | Put s p  => Get (fun s0 => Or (Put s (trans p)) (Put s0 Fail))
   end.
 
 Definition otrans {E A}: OProg E A -> OProg E A :=
@@ -657,14 +758,19 @@ Definition otrans {E A}: OProg E A -> OProg E A :=
 (* Translating contexts *)
 Fixpoint transC {E1 E2: list Type} {A B: Type} (c: Context E1 A E2 B) : Context E1 A E2 B :=
   match c in (Context E1 A E2 B) return (Context E1 A E2 B) with
-  | CHole           => CHole
-  | COr1 c q      => COr1 (transC c) (otrans q)
-  | COr2 p c      => COr2 (otrans p) (transC c)
-  | CPut v c       => CGet (fun s => true) (COr1 (CPut (fun env => v (tail env)) (CLift (transC c))) (fun env => Put (head env) Fail)) (fun s env => Fail)
-  | CGet t c q    => CGet t (transC c) (fun s => otrans (q s))
+  | CHole        => CHole
+  | COr1 c q     => COr1 (transC c) (otrans q)
+  | COr2 p c     => COr2 (otrans p) (transC c)
+  | CPut v c     => CGet (fun s => true)
+                         (COr1
+                            (CPut (fun env => v (tail env))
+                                  (CLift (transC c)))
+                            (fun env => Put (head env) Fail))
+                         (fun s env => Fail)
+  | CGet t c q   => CGet t (transC c) (fun s => otrans (q s))
   | CDelay t c q => CDelay t (transC c) (otrans q) 
   | CPush x c    => CPush x (transC c)
-  | CLift c         => CLift (transC c)
+  | CLift c      => CLift (transC c)
   end.
 
 Lemma otrans_cpush:
@@ -709,34 +815,31 @@ Lemma oevl_fail:
   forall {A E},
     @oevl A E (fun env => Fail) = fun env => failD.
 Proof.
-  intros; unfold oevl, orun, otrans; simpl; rewrite run_fail; auto.
+  auto.
 Qed.
 
 Lemma oevl_or:
   forall {A E} (p q: OProg E A),
     oevl (fun env => Or (p env) (q env)) = fun env => orD (oevl p env) (oevl q env).
 Proof.
-  intros; unfold oevl, orun, otrans; simpl; apply functional_extensionality; intro env; rewrite run_or; auto.
+  auto.
 Qed.
 
 Lemma oevl_get:
   forall {A E} (p: S -> OProg E A),
     oevl (fun env => Get (fun s => p s env)) = fun env => getD (fun s => oevl (p s) env).
 Proof.
-  intros; unfold oevl, orun, otrans; simpl; apply functional_extensionality; intro env; rewrite run_get; auto.
+  auto.
 Qed.
 
 Lemma oevl_put:
   forall {A E} (s: Env E -> S) (p: OProg E A),
     oevl (fun env => Put  (s env) (p env)) = fun env => getD (fun s0 => orD (putD (s env) (oevl p env)) (putD s0 failD)).
 Proof.
-  intros; unfold oevl, orun, otrans; simpl; apply functional_extensionality; intro env; rewrite run_get.
-  apply f_equal, functional_extensionality; intro s0. 
-  rewrite run_or; rewrite run_put. rewrite run_put; rewrite run_fail. auto.
+  auto.
 Qed.
 
 (* Proofs of the local state laws *)
-
 Lemma Meta1_Base:
   forall {A B E} (p q: OProg (A::E) B) 
     (P: forall {C D E'} (c: Context (A::(E)) C E' D) (k : B -> OProg (A::(E)) C), 
@@ -759,10 +862,10 @@ Proof.
           change (cpush a (obind ?p (fun x : B => clift (k x)))) with (appl (CPush a CHole)  (obind p (fun x : B => clift (k x)))).
           unfold oevl, orun, otrans in P. generalize env. apply equal_f; apply P.
      ** auto.
-     ** repeat rewrite run_or. rewrite (IHp0_1 p q), (IHp0_2 p q); auto.
-     ** repeat rewrite run_get. apply f_equal, functional_extensionality; intro x; rewrite (H x p q); auto.
-     ** repeat rewrite run_get; apply f_equal, functional_extensionality; intro s0. repeat rewrite run_or.
-         apply equal_f, f_equal. repeat rewrite run_put; apply f_equal; auto.
+     ** rewrite (IHp0_1 p q), (IHp0_2 p q); auto.
+     ** apply f_equal, functional_extensionality; intro x; rewrite (H x p q); auto.
+     ** apply f_equal, functional_extensionality; intro s0. 
+         apply equal_f, f_equal.  apply f_equal; auto.
 Qed.
 
 Lemma Meta1:
@@ -777,31 +880,31 @@ Proof.
   intros A B E p q P r C D E' c.
   dependent induction c; intros k env.
   - change (appl CHole ?p) with p. apply Meta1_Base; auto.
- - simpl. repeat rewrite oevl_or. rewrite (IHc p q); auto.
- - simpl. repeat rewrite oevl_or. rewrite (IHc p q); auto.
- - simpl. repeat rewrite oevl_put. rewrite (IHc p q); auto.
- - simpl. repeat rewrite oevl_get. apply f_equal; apply functional_extensionality; intro s0. 
+  - simpl. repeat rewrite oevl_or. rewrite (IHc p q); auto.
+  - simpl. repeat rewrite oevl_or. rewrite (IHc p q); auto.
+  - simpl. repeat rewrite oevl_put. rewrite (IHc p q); auto.
+  - simpl. repeat rewrite oevl_get. apply f_equal; apply functional_extensionality; intro s0. 
     destruct (b s0).
-   * unfold cpush, comap.
-     change (oevl (fun env0 => appl c ?p (Cons s0 env0)) env)
-         with (oevl (appl c p) (Cons s0 env)).
-  rewrite (IHc p q); auto.
-   * auto.
- - simpl. 
+    * unfold cpush, comap.
+      change (oevl (fun env0 => appl c ?p (Cons s0 env0)) env)
+        with (oevl (appl c p) (Cons s0 env)).
+      rewrite (IHc p q); auto.
+    * auto.
+  - simpl. 
     change (oevl
-  (fun env0 : Env E2 => if b env0 then ?p env0  else o env0)
-  env) with (oevl
-  (fun env0 : Env E2 => if b env then p env0 else o env0)
-  env).
+              (fun env0 : Env E2 => if b env0 then ?p env0  else o env0)
+              env) with (oevl
+                           (fun env0 : Env E2 => if b env then p env0 else o env0)
+                           env).
     destruct (b env).
     * apply IHc; auto.
     * auto.
- - simpl. unfold cpush, comap.
-   change (oevl (fun env0 : Env E2 => ?b (Cons c env0)) env) with (oevl b (Cons c env)).
-   apply IHc. auto.
- - simpl. unfold clift, comap.
+  - simpl. unfold cpush, comap.
+    change (oevl (fun env0 : Env E2 => ?b (Cons c env0)) env) with (oevl b (Cons c env)).
+    apply IHc. auto.
+  - simpl. unfold clift, comap.
     change (oevl (fun env0 => appl c ?p (tail env0)) env) with
-       (oevl (appl c p) (tail env)). auto. 
+        (oevl (appl c p) (tail env)). auto. 
 Qed.
 
 Lemma inverse_functional_extensionality:
@@ -972,6 +1075,10 @@ Proof.
   intros; unfold obind; simpl; apply put_get_L_1.
 Qed.
 
+(* TODO: ik wou dit bewijs even nader bekijken als voorbeeld van context/zcontext
+         switchen
+ASDF
+ *)
 Lemma put_fail_L_1:
   forall {E1 E2 A B} (c: Context E1 A E2 B) (v: Env E1 -> S),
     oevl (appl c (fun env => Put (v env) Fail))
@@ -981,7 +1088,7 @@ Proof.
   intros.
   unfold oevl; repeat rewrite otrans_appl; unfold otrans; simpl.
   repeat rewrite <- zappl_toZContext.
-  repeat rewrite invert_zappl_zget.
+  rewrite invert_zappl_zget.
   unfold clift, comap.
   repeat rewrite <- appl_fromZContext.
   rewrite put_or_G.
@@ -1021,137 +1128,137 @@ Proof.
   intros; unfold obind; simpl; apply put_fail_L_1.
 Qed.
 
+(* law 18 in the paper *)
+Lemma get_or : forall {A : Type} (p : S -> Prog A) (q : Prog A),
+    run (Get (fun s => Or (trans (p s)) q))
+    =
+    run (Or (Get (fun s => trans (p s))) q).
+Proof.
+  Admitted.
+
+
 Lemma put_or_trans:
   forall {E1 A} (p: OProg E1 A) {E2 B} (c: Context E1 A E2 B) (v: Env E1 -> S) (q: OProg E1 A),
     orun (appl c (fun env => Put (v env) (Or (otrans p env) (q env))))
     =
     orun (appl c (fun env => Or (Put (v env) (otrans p env)) (Put (v env) (q env)))).
 Proof.
-  intros E1 A p.
-  - intros E2 B c v q.
-    induction c; simpl.
-     * unfold orun, otrans; apply functional_extensionality; intro env. induction (p env); simpl.
-       -- rewrite put_ret_or_G.
-            rewrite <- (put_put_G' (v env) (v env) (q env)).
-            rewrite <- put_ret_or_G.
-           rewrite <- put_or_G'.
-           reflexivity.
-       -- rewrite run_put.
-            rewrite or_fail'.
-            rewrite put_or_G'.
-           rewrite run_put.
-           rewrite or_fail'.
-           repeat rewrite <- run_put.
-           rewrite put_put_G'.
-           reflexivity.
-       -- rewrite run_put.
-            rewrite or_or'.
-            rewrite <- run_put.
-            change (Or (trans p0_2) (q env)) with ((fun env => Or (trans p0_2) (q env)) env).
-            rewrite (IHp0_1(fun env => Or (trans p0_2) (q env))).
-            rewrite run_or.
-            rewrite IHp0_2.
-            rewrite <- run_or.
-            rewrite <- or_or'.
-            rewrite run_or.
-            change (trans p0_2) with ((fun env => trans p0_2) env) at 1.
-            rewrite <- IHp0_1.
-            rewrite <- run_or; auto.
-            auto.
-            auto.
-       -- repeat rewrite <- put_or_G'.
-            repeat rewrite run_or.
-            repeat rewrite put_get_G'. 
-            repeat rewrite <- run_or.
-            repeat rewrite put_or_G'.
-            rewrite H.
-            rewrite put_or_G'.
-            reflexivity.
-            auto.
-      -- repeat rewrite <- put_or_G'.
-           repeat rewrite run_or.
-           repeat rewrite put_get_G'.
-           repeat rewrite <- put_or_G'.
-           repeat rewrite run_or.
-           repeat rewrite put_put_G'.
-           repeat rewrite <- run_or.
-           repeat rewrite or_or'.
-           repeat rewrite run_or.
-           apply f_equal.
-           repeat rewrite <- run_or.
-           repeat rewrite put_or_G'.
-           repeat rewrite run_put.
-           repeat rewrite or_fail'.
-           repeat rewrite <- run_put.
-           rewrite put_put_G'.
-           reflexivity.
-    * unfold orun in *. apply functional_extensionality; intro env.
+  intros E1 A p E2 B c v q.
+  induction c; simpl.
+
+  (* Proof for empty context *)
+  - unfold orun, otrans; apply functional_extensionality; intro env. induction (p env). 
+    + simpl trans.
+      rewrite <- put_ret_or_G.
+      reflexivity.
+    + simpl trans.
+      rewrite put_or_G'.
+      change (run (Put ?s ?k)) with (putD s (run k)).
+      repeat rewrite or_fail'.
+      change (putD ?s (run ?p)) with (run (Put s p)).
+      rewrite put_put_G'.
+      reflexivity.
+    + simpl trans.
+      change (run (Put ?s ?p)) with (putD s (run p)).
+      rewrite or_or'.
+      rewrite <- run_put.
+      change (Or (trans p0_2) (q env)) with ((fun env => Or (trans p0_2) (q env)) env).
+      rewrite (IHp0_1(fun env => Or (trans p0_2) (q env))).
+      rewrite run_or.
+      rewrite IHp0_2; auto.
+      rewrite <- run_or.
+      rewrite <- or_or'.
+      rewrite run_or.
+      change (trans p0_2) with ((fun env => trans p0_2) env) at 1.
+      rewrite <- IHp0_1.
+      rewrite <- run_or; auto.
+      auto.
+    + simpl trans.
+
+      rewrite run_or.
+      rewrite put_get_G'.
+      rewrite <- run_or.
+
+      rewrite <- H; auto.
+
+      generalize (v env). intro.
+      change (Or (trans (p0 s)) (q env))
+        with ((fun s' => Or (trans (p0 s')) (q env)) s).
+      rewrite <- put_get_G'.
+
+      repeat rewrite run_put.
+      rewrite get_or.
+      reflexivity.
+
+    + simpl trans.
+      rewrite <- put_or_G'.
+
       repeat rewrite run_or.
-     assert (IHc' : forall (p : OProg E1 A) (v : Env E1 -> S) (q : OProg E1 A) (env: Env E2),
-      (run
-         (appl c (fun env0 : Env E1 => Put (v env0) (Or (otrans p env0) (q env0)))
-            env)) =
-      (run
-         (appl c
-            (fun env0 : Env E1 =>
-             Or (Put (v env0) (otrans p env0)) (Put (v env0) (q env0))) env))).
-         ** intros p0 v0 q0. apply equal_f. apply IHc.
-         ** rewrite IHc'. auto.
-   *  unfold orun in *. apply functional_extensionality; intro env.
-      repeat rewrite run_or.
-     assert (IHc' : forall (p : OProg E1 A) (v : Env E1 -> S) (q : OProg E1 A) (env: Env E2),
-      (run
-         (appl c (fun env0 : Env E1 => Put (v env0) (Or (otrans p env0) (q env0)))
-            env)) =
-      (run
-         (appl c
-            (fun env0 : Env E1 =>
-             Or (Put (v env0) (otrans p env0)) (Put (v env0) (q env0))) env))).
-         ** intros p0 v0 q0. apply equal_f. apply IHc.
-         ** rewrite IHc'. auto.
-   * unfold orun in *. apply functional_extensionality; intro env.
-     repeat rewrite run_put.
-       assert (IHc' : forall (p : OProg E1 A) (v : Env E1 -> S) (q : OProg E1 A) (env: Env E2),
-      (run
-         (appl c (fun env0 : Env E1 => Put (v env0) (Or (otrans p env0) (q env0)))
-            env)) =
-      (run
-         (appl c
-            (fun env0 : Env E1 =>
-             Or (Put (v env0) (otrans p env0)) (Put (v env0) (q env0))) env))).
-         ** intros p0 v0 q0. apply equal_f. apply IHc.
-         ** rewrite IHc'. auto.
-   *  unfold orun in *. apply functional_extensionality; intro env.
-     repeat rewrite run_get. apply f_equal; apply functional_extensionality; intro s0.
-     destruct (b s0).
-     -- unfold cpush, comap. 
-       assert (IHc' : forall (p : OProg E1 A) (v : Env E1 -> S) (q : OProg E1 A) (env: Env (S::E2)),
-      (run
-         (appl c (fun env0 : Env E1 => Put (v env0) (Or (otrans p env0) (q env0)))
-            env)) =
-      (run
-         (appl c
-            (fun env0 : Env E1 =>
-             Or (Put (v env0) (otrans p env0)) (Put (v env0) (q env0))) env))).
-         ** intros p0 v0 q0. apply equal_f. apply IHc.
-         ** rewrite IHc'. auto.
-   -- auto.
-  * change (orun (fun env => if b env then ?f env else ?g env))
-       with (fun env0 => orun (fun env => if b env0 then f env else g env) env0).
-     apply functional_extensionality; intro env0.
-     destruct (b env0).
-     ** rewrite IHc; auto.
-    ** auto. 
-  * unfold cpush, comap.
-    change (orun (fun env => ?f (Cons c env))) 
-      with (fun env => orun f (Cons c env)).
-      apply functional_extensionality; intro env.
-     rewrite IHc; auto.
-  * unfold clift, comap.
-        change (orun (fun env => ?f (tail env))) 
-      with (fun env => orun f (@tail C _ env)).
-      apply functional_extensionality; intro env.
-    rewrite IHc; auto.
+      rewrite put_get_G'.
+      repeat rewrite <- run_or.
+
+      rewrite put_or_G'; rewrite put_or_G'.
+      rewrite run_put; rewrite run_put.
+      repeat rewrite or_or'.
+      rewrite run_or.
+      rewrite put_or_G'.
+      rewrite run_or.
+      rewrite put_or_G'.
+      repeat rewrite run_put.
+      repeat rewrite or_fail'.
+      rewrite <- run_put.
+      rewrite <- run_put.
+      rewrite <- run_put.
+      rewrite put_put_G'.
+      reflexivity.
+
+  (* Proofs for non-empty context *)
+  - repeat rewrite orun_or.
+    apply functional_extensionality; intro.
+    change (orD ?t (orun o x)) with ((fun u => orD u (orun o x)) t).
+    f_equal.
+    rewrite IHc.
+    reflexivity.
+
+  - repeat rewrite orun_or.
+    apply functional_extensionality; intro env.
+    f_equal.
+    rewrite IHc.
+    reflexivity.
+
+  - repeat rewrite orun_put.
+    apply functional_extensionality; intro env.
+    f_equal.
+    rewrite IHc.
+    reflexivity.
+
+  - repeat rewrite orun_get.
+    apply functional_extensionality; intro env.
+    f_equal.
+    apply functional_extensionality; intro s.
+    destruct (b s); auto.
+    unfold cpush, comap.
+    unfold orun.
+    change (run (appl c ?p ?e)) with (orun (appl c p) e).
+    rewrite IHc.
+    reflexivity.
+
+  - unfold orun.
+    apply functional_extensionality; intro env.
+    destruct (b env); auto.
+    change (run (appl c ?p ?e)) with (orun (appl c p) e).
+    rewrite IHc.
+    reflexivity.
+    
+  - unfold orun, cpush, comap.
+    change (run (appl c0 ?p ?e)) with (orun (appl c0 p) e).
+    rewrite IHc.
+    reflexivity.
+
+  - unfold orun, clift, comap.
+    change (run (appl c ?p ?e)) with (orun (appl c p) e).
+    rewrite IHc.
+    reflexivity.
 Qed.
 
 Lemma get_put_L_1:
@@ -1160,7 +1267,7 @@ Lemma get_put_L_1:
     =
     oevl (appl c p).
 Proof.
-  intros; unfold oevl; repeat rewrite otrans_appl; unfold otrans; simpl.
+  intros. unfold oevl. repeat rewrite otrans_appl. unfold otrans. simpl.
   rewrite get_get_G.
   repeat rewrite <- zappl_toZContext.
   rewrite invert_zappl_zget.
@@ -1281,35 +1388,230 @@ Qed.
 *)
 
 Inductive BContext : list Type -> Type -> list Type -> Type -> Type :=
-  | BHole   : forall {E A}, BContext E A E A
-  | BOr1    : forall {E1 E2 A B}, BContext E1 A E2 B -> OProg E2 B -> BContext E1 A E2 B
-  | BOr2    : forall {E1 E2 A B}, OProg E2 B -> BContext E1 A E2 B -> BContext E1 A E2 B
-  | BPut     : forall {E1 E2 A B}, (Env E2 -> S) -> BContext E1 A E2 B -> BContext E1 A E2 B
-  | BGet     : forall {E1 E2 A B}, (S -> bool) -> (BContext E1 A (S::E2) B) -> (S -> OProg E2 B)-> BContext E1 A E2 B
-  | BDelay  : forall {E1 E2 A B}, (Env E2 -> bool) -> BContext E1 A E2 B -> OProg E2 B -> BContext E1 A E2 B
-  | BPush   : forall {E1 E2 A B C}, C -> BContext E1 A (C::E2) B-> BContext E1 A E2 B
-  | BLift      : forall {E1 E2 A B C}, BContext E1 A E2 B -> BContext E1 A (C::E2) B
-  | BBind1   : forall {E1 E2 A B C}, BContext E1 A E2 B -> (B -> OProg E2 C) -> BContext E1 A E2 C
-  | BBind2   : forall {E1 E2 A B C}, OProg E2 A -> BContext E1 B (A::E2) C -> BContext E1 B E2 C.
+  | BHole  : forall {E A}        , BContext E A E A
+
+  | BOr1   : forall {E1 E2 A B}  , BContext E1 A E2 B ->
+                                   OProg E2 B ->
+                                   BContext E1 A E2 B
+
+  | BOr2   : forall {E1 E2 A B}  , OProg E2 B ->
+                                   BContext E1 A E2 B ->
+                                   BContext E1 A E2 B
+
+  | BPut   : forall {E1 E2 A B}  , (Env E2 -> S) ->
+                                   BContext E1 A E2 B ->
+                                   BContext E1 A E2 B
+
+  | BGet   : forall {E1 E2 A B}  , (S -> bool) ->
+                                   (BContext E1 A (S::E2) B) ->
+                                   (S -> OProg E2 B) ->
+                                   BContext E1 A E2 B
+
+  | BDelay : forall {E1 E2 A B}  , (Env E2 -> bool) ->
+                                   BContext E1 A E2 B ->
+                                   OProg E2 B ->
+                                   BContext E1 A E2 B
+
+  | BPush  : forall {E1 E2 A B C}, C ->
+                                   BContext E1 A (C::E2) B ->
+                                   BContext E1 A E2 B
+
+  | BLift  : forall {E1 E2 A B C}, BContext E1 A E2 B ->
+                                   BContext E1 A (C::E2) B
+
+  (* [] >>= k
+     hole outputs B under environment E2
+     k outputs C under environment E2, given a B
+     current node produces this C, given environment E2
+     The whole program produces an A given E1
+   *)
+  | BBind1 : forall {E1 E2 A B C}, BContext E1 A E2 B ->
+                                   (B -> OProg E2 C) ->
+                                   BContext E1 A E2 C
+
+  (* m >>= \x -> []
+     m produces an A given E2 context
+     hole outputs a C under environment (A::E2)
+     current node produces this C given environment E2
+   *)
+  | BBind2 : forall {E1 E2 A B C}, OProg E2 A ->
+                                   BContext E1 B (A::E2) C ->
+                                   BContext E1 B E2 C.
+
+Inductive ZBContext : list Type -> Type -> list Type -> Type -> Type :=
+| ZBTop   : forall {E A}, ZBContext E A E A
+              
+| ZBOr1   : forall {E1 E2 A B}, ZBContext E1 A E2 B ->
+                                OProg E1 A ->
+                                ZBContext E1 A E2 B
+                                                   
+| ZBOr2   : forall {E1 E2 A B}, ZBContext E1 A E2 B ->
+                                OProg E1 A ->
+                                ZBContext E1 A E2 B
+                                                   
+| ZBPut   : forall {E1 E2 A B}, ZBContext E1 A E2 B ->
+                                (Env E1 -> S) ->
+                                ZBContext E1 A E2 B
+                                                      
+| ZBGet   : forall {E1 E2 A B}, ZBContext E1 A E2 B ->
+                                (S -> bool) ->
+                                (S -> OProg E1 A) ->
+                                ZBContext (S::E1) A E2 B
+                                                                         
+| ZBDelay : forall {E1 E2 A B}, ZBContext E1 A E2 B ->
+                                (Env E1 -> bool) ->
+                                OProg E1 A ->
+                                ZBContext E1 A E2 B
+                                                                       
+| ZBPush  : forall {E1 E2 A B C}, ZBContext E1 A E2 B ->
+                                  C ->
+                                  ZBContext (C::E1) A E2 B
+                                          
+| ZBLift  : forall {E1 E2 A B C}, ZBContext (C::E1) A E2 B ->
+                                  ZBContext E1 A E2 B
+        (* [] >>= k
+           hole outputs B under environment E2
+           k outputs C under environment E2, given a B
+           current node produces this C, given environment E2
+           The whole program produces an A given E1
+         *)
+
+(* [] >>= k *)
+(* hole produces an A under E1
+   k produces a B under same env, given an A
+   current node produces this B under environment E1
+   current node's parameters = first two of first ZBContext arg
+   whole program produces some unconstrained C under environment E2
+ *)
+| ZBBind1 : forall {E1 E2 A B C}, ZBContext E1 B E2 C ->
+                                  (A -> OProg E1 B) ->
+                                  ZBContext E1 A E2 C
+
+(* m >>= \x -> [] *)
+(* m produces an A under unextended environment E1 = OProg
+   hole produces a B under extended environment (A :: E1)
+   current node produces this B under environment E1
+   whole program produces some unconstrained C under environment E2
+    = last two of first arg
+ *)
+| ZBBind2 : forall {E1 E2 A B C}, ZBContext E1 B E2 C ->
+                                  OProg E1 A ->
+                                  ZBContext (A::E1) B E2 C.
+
 
 Fixpoint bappl {E1 E2: list Type} {A B: Type} (c: BContext E1 A E2 B)  : OProg E1 A -> OProg E2 B :=
   match c in (BContext E1 A E2 B) return (OProg E1 A -> OProg E2 B) with
-  | BHole => (fun p env => p env)
-  | BOr1 c q => (fun p env => Or (bappl c p env) (q env))
-  | BOr2 p c => (fun q env => Or (p env) (bappl c q env))
-  | BPut v c => (fun p env => Put (v env) (bappl c p env)) 
-  | BGet t c q => (fun p env => Get (fun s => if t s then cpush s (bappl c p) env else q s env))
+  | BHole        => (fun p env => p env)
+  | BOr1 c q     => (fun p env => Or (bappl c p env) (q env))
+  | BOr2 p c     => (fun q env => Or (p env) (bappl c q env))
+  | BPut v c     => (fun p env => Put (v env) (bappl c p env)) 
+  | BGet t c q   => (fun p env => Get (fun s =>
+                                         if t s then cpush s (bappl c p) env else q s env))
   | BDelay t c q => (fun p => (fun env => if t env then bappl c p env else q env))
-  | BPush x c => (fun p env => cpush x (bappl c p) env)
-  | BLift c => (fun p env => clift (bappl c p) env)
-  | BBind1 c k => (fun p env => bind (bappl c p env) (fun x => k x env))
-  | BBind2 p c => (fun q env => bind (p env) (fun x => cpush x (bappl c q) env))
+  | BPush x c    => (fun p env => cpush x (bappl c p) env)
+  | BLift c      => (fun p env => clift (bappl c p) env)
+  | BBind1 c k   => (fun p env => bind (bappl c p env) (fun x => k x env))
+  | BBind2 p c   => (fun q env => bind (p env) (fun x => cpush x (bappl c q) env))
   end.
+
+Fixpoint zbappl {E1 E2: list Type} {A B : Type} (z: ZBContext E1 A E2 B) : OProg E1 A -> OProg E2 B :=
+  match z in (ZBContext E1 A E2 B) return (OProg E1 A -> OProg E2 B) with
+  | ZBTop         => (fun p env => p env)
+  | ZBOr1 z q     => (fun p     => zbappl z (fun env => Or (p env) (q env)))
+  | ZBOr2 z p     => (fun q     => zbappl z (fun env => Or (p env) (q env)))
+  | ZBPut z v     => (fun p     => zbappl z (fun env => Put (v env) (p env)))
+  | ZBGet z t q   => (fun p     =>
+                        zbappl z (fun env =>
+                                   Get (fun s => if t s
+                                                 then (cpush s p) env
+                                                 else q s env)))
+  | ZBDelay z t q => (fun p     =>
+                        zbappl z (fun env =>
+                                    if t env then p env else q env))
+  | ZBPush z c    => (fun p     => zbappl z (cpush c p))
+  | ZBLift z      => (fun p     => zbappl z (clift p))
+(* p : OProg E1 A
+   zbappl z: OProg E1 A -> OProg E2 B
+ *)
+  | ZBBind1 z k => fun p => zbappl z (fun env => bind (p env) (fun x => k x env))
+  | ZBBind2 z m => fun p => zbappl z (fun env =>
+                                        bind (m env) (fun x => cpush x p env))
+  end.
+
+Fixpoint toZBContext_ {E1 E2 A B} (c: BContext E1 A E2 B):
+  (forall {E3 C}, ZBContext E2 B E3 C -> ZBContext E1 A E3 C) :=
+  match c in (BContext E1 A E2 B) return ((forall {E3 C}, ZBContext E2 B E3 C-> ZBContext E1 A E3 C)) with
+   | BHole        => (fun _ _ z => z)
+   | BOr1 c p     => (fun _ _ z => toZBContext_ c (ZBOr1 z p))
+   | BOr2 p c     => (fun _ _ z => toZBContext_ c (ZBOr2 z p))
+   | BPut s c     => (fun _ _ z => toZBContext_ c (ZBPut z s))
+   | BGet t c p   => (fun _ _ z => toZBContext_ c (ZBGet z t p))
+   | BDelay t c p => (fun _ _ z => toZBContext_ c (ZBDelay z t p))
+   | BPush a c    => (fun _ _ z => toZBContext_ c (ZBPush z a))
+   | BLift c      => (fun _ _ z => toZBContext_ c (ZBLift z))
+   | BBind1 c k   => (fun _ _ z => toZBContext_ c (ZBBind1 z k))
+   | BBind2 p c   => (fun _ _ z => toZBContext_ c (ZBBind2 z p))
+  end.
+
+Definition toZBContext {E1 E2 A B} (c: BContext E1 A E2 B): ZBContext E1 A E2 B := toZBContext_ c ZBTop.
+ 
+Lemma zbappl_toZBContext_:
+   forall {E1 E2 A B} (c: BContext E1 A E2 B) {E3 C} (z: ZBContext E2 B E3 C) (p: OProg E1 A),
+     zbappl (toZBContext_ c z) p = zbappl z (bappl c p).
+Proof.
+  intros E1 E2 A B c; induction c; intros E3 D z prog; simpl; auto; rewrite IHc; auto.
+Qed.
+
+Lemma zbappl_toZBContext:
+   forall {E1 E2 A B} (c: BContext E1 A E2 B) (p: OProg E1 A),
+     zbappl (toZBContext c) p = bappl c p.
+Proof.
+  intros; unfold toZBContext; rewrite zbappl_toZBContext_; simpl; reflexivity.
+Qed.
+
+(*
+Lemma invert_zappl_zput:
+  forall {E1 E2 A B} (z: ZContext E1 A E2 B) (v: Env E1 -> S) (q: OProg E1 A),
+     zappl z (fun env => Put (v env) (q env))
+     =
+     zappl (ZPut z v) q.
+Proof.
+  intros; simpl; unfold cpush, clift, comap, head, tail, head_, tail_; auto.
+Qed.
+
+Lemma invert_zappl_zor2:
+  forall {E1 E2 A B} (z: ZContext E1 A E2 B)  (p q: OProg E1 A),
+     zappl z (fun env => Or (p env) (q env))
+     =
+     zappl (ZOr2 z p) q.
+Proof.
+  intros; simpl; unfold cpush, clift, comap, head, tail, head_, tail_; auto.
+Qed.
+
+Lemma invert_zappl_zget:
+  forall {E1 E2 A B} (z: ZContext E1 A E2 B)  (p: S -> OProg E1 A),
+     zappl z (fun env => Get (fun s => p s env))
+     =
+     zappl (ZGet z (fun _ => true) (fun _ _ => Fail)) (fun env' => clift (p (head env')) env').
+Proof.
+  intros; simpl; unfold cpush, clift, comap, head, tail, head_, tail_; auto.
+Qed.
+
+Lemma invert_zappl_zget_or:
+  forall {E1 E2 A B} (z: ZContext E1 A E2 B)  (p q: S -> OProg E1 A),
+     zappl z (fun env => Get (fun s => Or (p s env) (q s env)))
+     =
+     zappl (ZOr1 (ZGet z (fun _ => true) (fun _ _ => Fail)) (fun env' => clift (q (head env')) env')) (fun env' => clift (p (head env')) env').
+Proof.
+  intros; simpl; unfold cpush, clift, comap, head, tail, head_, tail_; auto.
+Qed.
+*)
 
 Lemma bappFromAppl:
   forall {A B E1 E2} (p q: OProg E1 A)
-    (P: forall {C E2 B} (c: Context E1 C E2 B) (k: A -> OProg E1 C), oevl (appl c (obind p k)) = oevl (appl c (obind q k)))
-    (b: BContext E1 A E2 B) ,
+    (P: forall {C E2 B} (c: Context E1 C E2 B) (k: A -> OProg E1 C),
+        oevl (appl c (obind p k)) = oevl (appl c (obind q k)))
+    (b: BContext E1 A E2 B),
     oevl (bappl b p) = oevl (bappl b q).
 Proof.
   intros a B E1 E2 p q P b.
@@ -1339,7 +1641,27 @@ Proof.
      change (oevl (fun env : Env (C :: E2) => bappl b ?p (tail env))) with
                 (fun env0 => oevl (bappl b p) (@tail C _ env0)).
     rewrite (IHb p q); auto.
-  - admit. (* TODO: need zipper-variant of BContext *)
+  -
+    (*
+    apply functional_extensionality; intro env0.
+    change (oevl (fun env => bind (bappl b ?r env) (fun x => o x env)) env0)
+      with (oevl (fun env => bind (bappl b r env0) (fun x => o x env0)) env0).
+
+    unfold oevl, otrans, obind, orun.
+    
+    change (run (trans ?prog))
+      with (evl prog).
+
+
+    change (fun env => bind (bappl b ?r env) (fun x => o x env))
+      with (obind (bappl b r) o).
+
+
+    apply IHb in P.
+    change (bind (bappl b p ?env) ?k)
+      with (bappl (BBind1 b k) p env).
+*)
+    admit. (* TODO: need zipper-variant of BContext *)
   - admit. (* TODO: need zipper-variant of BContext *)
 Admitted.
 
@@ -1363,11 +1685,11 @@ Definition failD : forall {A}, D A :=
 
 Definition orD : forall {A}, D A -> D A -> D A :=
   fun A xs ys => 
-      (fun s => match xs s with
-                     | (ansx, s') => match ys s' with
-                                         | (ansy, s'') => (ansx ++ ansy, s'')
-                                         end
-                     end).
+    (fun s => match xs s with
+              | (ansx, s') => match ys s' with
+                              | (ansy, s'') => (ansx ++ ansy, s'')
+                              end
+              end).
 
 Definition getD : forall {A}, (S -> D A) -> D A :=
   fun A k => 
